sel4_artifacts/UxASSeL4/verification/WaypointManagerUtils.h
@@ -1,33 +1,37 @@
-#ifndef __MISSIONCOMMANDUTILS_H__
-#define __MISSIONCOMMANDUTILS_H__
+/*
+ * Author: Dan DaCosta
+ * Company: Rockwell Collins
+ * License: Air Force Open Source Agreement Version 1.0
+ *
+ * Terminology: 
+ *
+ *  waypoint - Largely self-explanatory. We are only really using the number
+ *  and nextwaypoint field in this data structure.
+ *
+ *  mission command - An array of unordered Waypoint data
+ *  structures.
+ *
+ *  mission command segment - An array of unordered Waypoint data
+ *  structure which is a subset of a mission command.
+ *   
+ */
+#ifndef __WAYPOINTMANAGERUTILS_H__
+#define __WAYPOINTMANAGERUTILS_H__
 #include <stdbool.h>
-/*#include "MissionCommand.h"*/
-#include "Waypoint.h"
+#include "../CMASI/Waypoint.h"
 
-int lmcp_process_msg(uint8_t** inb, size_t size, lmcp_object **o);
-int lmcp_unpack(uint8_t** inb, size_t size, lmcp_object **o);
-
-
-/*struct MissionCommandExt_struct{
-  MissionCommand missioncommand;
-  Waypoint * waypoints;
-  uint16_t waypointslen;
-
-};
-
-typedef struct MissionCommandExt_struct MissionCommandExt; 
-
-void MCEInit(MissionCommandExt * mce, uint16_t waypoints);*/
-Waypoint * FindWP(Waypoint * ws, uint16_t len, int64_t id);
-void MCWaypointSubSequence(  Waypoint * ws
-                           , uint16_t len_ws
-                           , int64_t id
-                           , uint16_t len_ws_win
-                             , Waypoint * ws_win /* out */);
-bool GetMCWaypointSubSequence( Waypoint * ws
-                             , uint16_t len_ws
-                             , int64_t last_start_id
-                             , int64_t approach_id
-                             , uint16_t len_ws_win
-                               , Waypoint * ws_win /* out */ );
-#endif /* __MISSIONCOMMANDUTILS_H__ */
+void AutoPilotMissionCommandSegment( Waypoint * ws /* mission
+                                                      command. */
+                                     , uint16_t len_ws /* mission
+                                                          command
+                                                          length. */
+                                     , int64_t id /* starting ID for
+                                                     mission command
+                                                     segment. */
+                                     , Waypoint * ws_win /* mission command segment */ /* out */
+                                     , uint16_t len_ws_win /* mission
+                                                              command
+                                                              segment
+                                                              length */
+                                     );
+#endif /* __WAYPOINTMANAGERUTILS_H__ */
