sel4_artifacts/UxASSeL4/verification/ImplToFunSpec.thy
@@ -107,13 +107,13 @@ lemma findwp_success_aux[wp]:
   \<and> are_valid_Waypoints s wsp len
   \<and> (\<exists> w. Some w = find_waypoint (lift_waypoints s wsp len) i)
   \<and> P s\<rbrace>
-   LoadCode.MissionCommandUtils.FindWP' wsp len i
+   LoadCode.WaypointManagerUtils.FindWaypoint' wsp len i
 \<lbrace> \<lambda> r s. are_valid_Waypoints s wsp len
   \<and> Some (heap_Waypoint_struct_C s r) = find_waypoint (lift_waypoints s wsp len) i 
   \<and> is_valid_Waypoint_struct_C s r 
   \<and> P s \<rbrace>!"
   apply (rule validNF_assume_pre)
-  apply (unfold LoadCode.MissionCommandUtils.FindWP'_def)
+  apply (unfold LoadCode.WaypointManagerUtils.FindWaypoint'_def)
   apply (unfold skipE_def)
   apply wp
   apply(subst whileLoopE_add_inv
@@ -145,7 +145,7 @@ g r
 (\<forall> s. P s \<longrightarrow>  len \<le> USHORT_MAX  \<and> are_valid_Waypoints s wsp len \<and> (\<exists> w. Some w = find_waypoint (lift_waypoints s wsp len) i)) 
 \<Longrightarrow>
 \<lbrace> P \<rbrace> 
-do x \<leftarrow> MissionCommandUtils.FindWP' wsp len i; 
+do x \<leftarrow> WaypointManagerUtils.FindWaypoint' wsp len i; 
         g x 
 od 
 \<lbrace> Q \<rbrace>!"    
@@ -160,15 +160,10 @@ lemma validNF_guard_bind[wp]:"\<lbrace>\<lambda> s. A s \<and> f s\<rbrace> g ()
   apply (rule validNF_bind[where B="\<lambda> _ s. A s \<and> f s"])
   by (wp | auto)+
     
-lemma validNF_whileloop_inv[wp]:"\<forall> r. \<lbrace> \<lambda> s. P s \<and> i r s \<and> \<not> (c r s) \<rbrace> g r \<lbrace> Q \<rbrace>!
-\<Longrightarrow> \<lbrace> P \<rbrace> whileLoop_inv c s v i m \<lbrace> \<lambda> r s. P s \<and> i r s \<and> \<not>(c r s) \<rbrace>!  
-\<Longrightarrow> \<lbrace> P \<rbrace> do x \<leftarrow> whileLoop_inv c s v i m; g x od \<lbrace> Q \<rbrace>!"
-  apply (rule validNF_bind[where B = "\<lambda> r s. P s \<and> i r s \<and> \<not>(c r s)"])
-  by auto
-    
-lemma validNF_modify[wp]:"\<forall> s'. \<lbrace> \<lambda> s. P s \<and> s = f s' \<rbrace> g \<lbrace> Q \<rbrace>! \<Longrightarrow> \<lbrace> \<lambda> s. P s\<rbrace> do x \<leftarrow> modify f; g od \<lbrace> Q \<rbrace>!"
-  sorry
-    
+
+lemma validNF_modify[wp]:"\<forall> s'. \<lbrace> \<lambda> s. P s' \<and> s = f s' \<rbrace> g \<lbrace> Q \<rbrace>! \<Longrightarrow> \<lbrace> P \<rbrace> do x \<leftarrow> modify f; g od \<lbrace> Q \<rbrace>!"
+sorry
+  
 lemma forward_validNF_gets[wp]:"\<forall> x. \<lbrace> \<lambda> s. P s \<and> x = f s \<rbrace> g x \<lbrace> Q \<rbrace>! \<Longrightarrow> \<lbrace> P \<rbrace> do x \<leftarrow> gets f; g x od \<lbrace> Q \<rbrace>!"
   apply (rule validNF_bind[where B="\<lambda> x s. P s \<and> x = f s"])
    apply blast
@@ -183,31 +178,34 @@ lemma validNF_nobind[wp]:"\<lbrace>B\<rbrace> g \<lbrace>C\<rbrace>! \<Longright
 lemma are_valid_waypoints_noninter[simp]:"are_valid_Waypoints (heap_Waypoint_struct_C_update f s) p2 len = are_valid_Waypoints s p2 len"
   apply (unfold are_valid_Waypoints_def) by auto
 
-lemma rename8[simp]:"x \<noteq> y \<Longrightarrow> heap_Waypoint_struct_C (heap_Waypoint_struct_C_update (\<lambda>b c. if c = x then v else b c) s') y = heap_Waypoint_struct_C s' y"
-  by auto
-    
+(*
 (* TODO: How do I prove this *)
 lemma base_Waypoint_struct_C_ptr_ineq:"(p::Waypoint_struct_C ptr) +\<^sub>p (1::nat) \<noteq> p" 
   sorry
 (* TODO: How do I prove this *)
 lemma general_Waypoint_struct_C_ptr_ineq:"0<(x::nat)  \<Longrightarrow> (p::Waypoint_struct_C ptr) +\<^sub>p  x  \<noteq> p "   
   sorry
+
+theorem "size_td (typ_info_t TYPE(Waypoint_struct_C)) = x"
+  apply simp
+
+ *)  
     
 lemma MCWaypointSubSequence_to_funspec_supp1:
-assumes a2:"Some win  = waypoints_window_aux ws i len"
-and a3:"int a < int len"
-and a4:"a = 0 \<longrightarrow> b = sint i"
-and a5:"0 < a \<longrightarrow> b = sint (nextwaypoint_C (win ! (a - Suc 0)))"
-shows "\<exists>w. Some w = find_waypoint ws (of_int b)"
-proof -
+assumes a2:"Some win = waypoints_window_aux (lift_waypoints s wsp len_ws) i len_ws_win"
+and a8:"a = 0 \<longrightarrow> b = sint i"
+and a9:"0 < a \<longrightarrow> b = sint (nextwaypoint_C (win ! (a - Suc 0)))"
+and a11:"a < len_ws_win" 
+shows "Some (win ! a) = find_waypoint (lift_waypoints s wsp len_ws) (of_int b)"
+proof - 
   have "a = 0 \<or> 0 < a" by auto
   thus ?thesis
-  proof 
+  proof
     assume "a = 0"
-    thus ?thesis by (metis a2 a4 of_int_sint waypoint_window_aux_find_waypoint_hd)
+    thus ?thesis using a11 a2 a8 waypoint_window_aux_nextwp by auto
   next
     assume "0 < a"
-    thus ?thesis using a2 a3 a5 waypoint_window_aux_nextwp by force
+    thus ?thesis using a11 a2 a9 waypoint_window_aux_nextwp by auto
   qed
 qed
     
@@ -232,80 +230,33 @@ proof -
    qed
 qed
 
-lemma MCWaypointSubSequence_to_funspec_supp3:
-assumes a4:"Some win =
-                waypoints_window_aux
-                 (lift_waypoints (heap_Waypoint_struct_C_update (\<lambda>b c. if c = wsp +\<^sub>p int len_ws +\<^sub>p int a then heap_Waypoint_struct_C s' r else b c) s') wsp len_ws) i
-                 len_ws_win"
-and a8:"Some (heap_Waypoint_struct_C s' r) =
-                find_waypoint (lift_waypoints (heap_Waypoint_struct_C_update (\<lambda>b c. if c = wsp +\<^sub>p int len_ws +\<^sub>p int a then heap_Waypoint_struct_C s' r else b c) s') wsp len_ws)
-                 (of_int b)"
-and a12:"a = 0 \<longrightarrow> b = sint i"
-and a13:"0 < a \<longrightarrow> b = sint (nextwaypoint_C (win ! (a - Suc 0)))"
-and a15:"a < len_ws_win"
-shows "nextwaypoint_C (heap_Waypoint_struct_C s' r) = nextwaypoint_C (win ! a)"
+lemma MCWaypointSubSequence_to_funspec_supp4:
+assumes a1:"len_ws \<le> USHORT_MAX"
+and a2:"Some win = waypoints_window_aux (lift_waypoints s' wsp len_ws) i len_ws_win"
+and a3:"len_ws_win \<le> len_ws"
+and a6:"Some (heap_Waypoint_struct_C s' r) = find_waypoint (lift_waypoints s' wsp len_ws) (of_int b)"
+and a10:"a = 0 \<longrightarrow> b = sint i"
+and a11:"0 < a \<longrightarrow> b = sint (nextwaypoint_C (win ! (a - Suc 0)))"
+and a13:"a < len_ws_win"
+and a14:"wsp +\<^sub>p int len_ws +\<^sub>p int k = wsp +\<^sub>p int len_ws +\<^sub>p int a"
+and a15:"k \<le> a"
+shows "heap_Waypoint_struct_C s' r = win ! k"  
 proof -
-  have "a = 0 \<or> 0 < a" by auto
+  have y1:"a \<le> USHORT_MAX"  using a1 a13 a3 by auto 
+  have y2:"k \<le> USHORT_MAX"  using a15 y1 by auto
+  have y3:"a = k" using ptr_offset_equality a14 y1 y2 by fastforce
+  then have " a = 0 \<or> 0 < a" by auto
   thus ?thesis
-  proof
+  proof 
     assume "a = 0"
     thus ?thesis
-      by (metis (no_types, lifting) a12 a4 a8 hd_conv_nth of_int_sint option.inject waypoint_window_aux_find_waypoint_hd waypoint_window_aux_success_len_nonempty)
+      by (metis a10 a2 a6 hd_conv_nth of_int_sint option.inject waypoint_window_aux_find_waypoint_hd waypoint_window_aux_success_len_nonempty y3)
   next
     assume "0 < a"
-    thus ?thesis by (metis (no_types, lifting) One_nat_def a13 a15 a4 a8 of_int_sint option.inject waypoint_window_aux_nextwp)
+    thus ?thesis
+      by (metis One_nat_def a11 a13 a2 a6 of_int_sint option.inject waypoint_window_aux_nextwp y3)
   qed
 qed
-
-lemma MCWaypointSubSequence_to_funspec_supp4_old:
-assumes a4:"Some win =
-       waypoints_window_aux (lift_waypoints (heap_Waypoint_struct_C_update (\<lambda>b c. if c = wsp +\<^sub>p int len_ws +\<^sub>p int a then heap_Waypoint_struct_C s' r else b c) s') wsp len_ws) i
-        len_ws_win"
-and a8:"Some (heap_Waypoint_struct_C s' r) =
-       find_waypoint (lift_waypoints (heap_Waypoint_struct_C_update (\<lambda>b c. if c = wsp +\<^sub>p int len_ws +\<^sub>p int a then heap_Waypoint_struct_C s' r else b c) s') wsp len_ws)
-        (of_int b)"
-and a12:"a = 0 \<longrightarrow> b = sint i"
-and a13:"0 < a \<longrightarrow> b = sint (nextwaypoint_C (win ! (a - Suc 0)))"
-and a14:"\<forall>k\<le>a - Suc 0.
-          0 < a \<longrightarrow>
-          (if wsp +\<^sub>p int len_ws +\<^sub>p int k = wsp +\<^sub>p int len_ws +\<^sub>p int a then heap_Waypoint_struct_C s' r else heap_Waypoint_struct_C s' (wsp +\<^sub>p int len_ws +\<^sub>p int k)) =
-          win ! k"
-and a15:"a < len_ws_win"
-and a16:"wsp +\<^sub>p int len_ws +\<^sub>p int k = wsp +\<^sub>p int len_ws +\<^sub>p int a"
-and a17:"k \<le> a"
-shows "heap_Waypoint_struct_C s' r = win ! k"
-proof -
-  have "k = a \<or> k < a" using a17 by auto
-  thus ?thesis
-  proof
-    assume y1:"k = a"
-   thus ?thesis by (metis (no_types, lifting) One_nat_def a12 a13 a15 a4 a8 not_gr_zero of_int_sint option.inject waypoint_window_aux_nextwp)          
-  next 
-    assume y1:"k < a"
-    then have "k \<le> a - Suc 0" by auto
-    thus ?thesis using a14 a16 y1 by auto
-  qed
-qed
-  
-lemma MCWaypointSubSequence_to_funspec_supp4:"len_ws \<le> USHORT_MAX \<Longrightarrow>
-       ws_winp = wsp +\<^sub>p int len_ws \<Longrightarrow>
-       Some win = waypoints_window_aux (lift_waypoints s' wsp len_ws) i len_ws_win \<Longrightarrow>
-       len_ws_win < len_ws \<Longrightarrow>
-       \<forall>s v a. a < len_ws_win \<longrightarrow>
-               lift_waypoints (heap_Waypoint_struct_C_update (\<lambda>b c. if c = wsp +\<^sub>p int len_ws +\<^sub>p int a then v else b c) s) wsp len_ws = lift_waypoints s wsp len_ws \<Longrightarrow>
-       are_valid_Waypoints s' wsp len_ws \<Longrightarrow>
-       Some (heap_Waypoint_struct_C s' r) = find_waypoint (lift_waypoints s' wsp len_ws) (of_int b) \<Longrightarrow>
-       is_valid_Waypoint_struct_C s' r \<Longrightarrow>
-       are_valid_Waypoints s' (wsp +\<^sub>p int len_ws) len_ws_win \<Longrightarrow>
-       ws = lift_waypoints s' wsp len_ws \<Longrightarrow>
-       a = 0 \<longrightarrow> b = sint i \<Longrightarrow>
-       0 < a \<longrightarrow> b = sint (nextwaypoint_C (win ! (a - Suc 0))) \<Longrightarrow>
-       \<forall>k\<le>a - Suc 0.
-          0 < a \<longrightarrow>
-          (if wsp +\<^sub>p int len_ws +\<^sub>p int k = wsp +\<^sub>p int len_ws +\<^sub>p int a then heap_Waypoint_struct_C s' r else heap_Waypoint_struct_C s' (wsp +\<^sub>p int len_ws +\<^sub>p int k)) =
-          win ! k \<Longrightarrow>
-       a < len_ws_win \<Longrightarrow> wsp +\<^sub>p int len_ws +\<^sub>p int k = wsp +\<^sub>p int len_ws +\<^sub>p int a \<Longrightarrow> k \<le> a \<Longrightarrow> heap_Waypoint_struct_C s' r = win ! k"  
-  sorry
 
 lemma MCWaypointSubSequence_to_funspec_supp5:
 assumes a14:"\<forall>k\<le>a - Suc 0.
@@ -331,107 +282,143 @@ qed
 lemma lift_lift_waypoint_agnostic_prop:
 "a < len_ws_win
 \<Longrightarrow> \<forall>(s::lifted_globals) v a. a < len_ws_win \<longrightarrow>
-                        lift_waypoints (heap_Waypoint_struct_C_update (\<lambda>b c. if c = wsp +\<^sub>p int len_ws +\<^sub>p int a then v else b c) s) wsp len_ws = lift_waypoints s wsp len_ws
+                        lift_waypoints (heap_Waypoint_struct_C_update (\<lambda>b c. if c = wsp +\<^sub>p int len_ws +\<^sub>p int a then v b else b c) s) wsp len_ws = lift_waypoints s wsp len_ws
 \<Longrightarrow>
-lift_waypoints (heap_Waypoint_struct_C_update (\<lambda>b c. if c = wsp +\<^sub>p int len_ws +\<^sub>p int a then v else b c) (s::lifted_globals)) wsp len_ws = lift_waypoints s wsp len_ws"
+lift_waypoints (heap_Waypoint_struct_C_update (\<lambda>b c. if c = wsp +\<^sub>p int len_ws +\<^sub>p int a then v b else b c) (s::lifted_globals)) wsp len_ws = lift_waypoints s wsp len_ws"
 by auto
 
-(*
-theorem "size_td (typ_info_t TYPE(Waypoint_struct_C)) = x"
-  apply simp
-
- *)  
-lemma FillWaypoint_to_funspec:
+lemma FillWindow_to_funspec:
 "len_ws \<le> USHORT_MAX
-\<Longrightarrow> ws_winp = wsp +\<^sub>p len_ws
 \<Longrightarrow> Some win = waypoints_window_aux ws i len_ws_win
-\<Longrightarrow> len_ws_win < len_ws 
+\<Longrightarrow> len_ws_win \<le> len_ws 
 \<Longrightarrow> 0<len_ws_win
-\<Longrightarrow> (\<forall> (s::lifted_globals) v a. a < len_ws_win  \<longrightarrow> lift_waypoints (heap_Waypoint_struct_C_update (\<lambda>b c. if c = ws_winp +\<^sub>p int a then v else b c) s) wsp len_ws = lift_waypoints s wsp len_ws)
+\<Longrightarrow> (\<forall> (s::lifted_globals) v a. a < len_ws_win  \<longrightarrow> lift_waypoints (heap_Waypoint_struct_C_update (\<lambda>b c. if c =  wsp +\<^sub>p len_ws +\<^sub>p int a then v b else b c) s) wsp len_ws = lift_waypoints s wsp len_ws)
 \<Longrightarrow> \<lbrace>\<lambda> (s::lifted_globals).
-  are_valid_Waypoints s ws_winp len_ws_win
+  are_valid_Waypoints s ( wsp +\<^sub>p len_ws) len_ws_win
   \<and> are_valid_Waypoints s wsp len_ws
   \<and> ws = lift_waypoints s wsp len_ws \<rbrace>
-  LoadCode.MissionCommandUtils.FillWindow' wsp len_ws i len_ws_win ws_winp
+  LoadCode.WaypointManagerUtils.FillWindow' wsp len_ws i len_ws_win ( wsp +\<^sub>p len_ws)
 \<lbrace> \<lambda> r s. 
-  are_valid_Waypoints s ws_winp len_ws_win
+  are_valid_Waypoints s ( wsp +\<^sub>p len_ws) len_ws_win
   \<and> are_valid_Waypoints s wsp len_ws
   \<and> ws = lift_waypoints s wsp len_ws
-  \<and> (\<forall> j. j <  len_ws_win \<longrightarrow> heap_Waypoint_struct_C s (ws_winp +\<^sub>p j) = win ! j) \<rbrace>!"
-  apply (unfold LoadCode.MissionCommandUtils.FillWindow'_def)
+  \<and> (\<forall> j. j <  len_ws_win \<longrightarrow> heap_Waypoint_struct_C s ( wsp +\<^sub>p len_ws +\<^sub>p j) = win ! j) \<rbrace>!"
+  apply (unfold LoadCode.WaypointManagerUtils.FillWindow'_def)
       apply(subst whileLoop_add_inv
         [where 
           M = "\<lambda> ((j,nid),s). len_ws_win - j"
           and I = 
             "\<lambda> (j,nid) s.
-  are_valid_Waypoints s ws_winp len_ws_win
+  are_valid_Waypoints s  (wsp +\<^sub>p len_ws) len_ws_win
   \<and>  are_valid_Waypoints s wsp len_ws
   \<and> ws = lift_waypoints s wsp len_ws
   \<and> j \<le> len_ws_win
 \<and> (j = 0 \<longrightarrow> nid = sint i)
 \<and> (0 < j \<longrightarrow> nid = sint (nextwaypoint_C (win ! (j - 1))))
-\<and> (\<forall> k \<le> j - 1. 0 < j \<longrightarrow> heap_Waypoint_struct_C s (ws_winp +\<^sub>p k) = win ! k)
-" ])
-  apply ( assumption 
+\<and> (\<forall> k \<le> j - 1. 0 < j \<longrightarrow> heap_Waypoint_struct_C s ( wsp +\<^sub>p len_ws +\<^sub>p k) = win ! k)
+" ])        
+  by ( assumption 
       | clarsimp  
       | wp_once 
       | simp add: lift_lift_waypoint_agnostic_prop 
-                  MCWaypointSubSequence_to_funspec_supp2)+
-         apply rule+
-    
-           apply (rule MCWaypointSubSequence_to_funspec_supp4)   
-            apply(assumption | clarsimp)+
-          apply(rule MCWaypointSubSequence_to_funspec_supp5)
-     apply(assumption | clarsimp)+
-                      apply (assumption | simp add: MCWaypointSubSequence_to_funspec_supp1 | clarsimp)+
-  done
-    
-lemma foo:"
-Some win' = waypoints_window_aux ws i len_ws_win \<Longrightarrow>
+                  MCWaypointSubSequence_to_funspec_supp2
+      | rule
+      | rule MCWaypointSubSequence_to_funspec_supp1 
+             MCWaypointSubSequence_to_funspec_supp2 
+             MCWaypointSubSequence_to_funspec_supp4 
+             MCWaypointSubSequence_to_funspec_supp5 
+      | linarith)+ (* Takes a little while *)
+
+        
+lemma GroomWindow_to_funspec_supp1:
+  assumes a2:"Some win' = waypoints_window_aux ws i len_ws_win"
+and a3:"wsp +\<^sub>p int len_ws +\<^sub>p int j = wsp +\<^sub>p int len_ws +\<^sub>p (int len_ws_win - 1)"
+and a4:"j < len_ws_win"
+and a5:"len_ws_win \<le> USHORT_MAX"
+and a6:"(\<forall> j. j <  len_ws_win \<longrightarrow> heap_Waypoint_struct_C s (wsp +\<^sub>p len_ws +\<^sub>p j) = win' ! j)"
+and a7:"Some win = waypoints_window ws i len_ws_win"
+shows "nextwaypoint_C_update (\<lambda>a. number_C (heap_Waypoint_struct_C s (wsp +\<^sub>p int len_ws +\<^sub>p (int len_ws_win - 1))))
+                (heap_Waypoint_struct_C s (wsp +\<^sub>p int len_ws +\<^sub>p (int len_ws_win - 1))) =
+               win ! j"
+proof -
+  have y1:"len_ws_win - 1 \<le> USHORT_MAX" using a5 by auto
+  have y2:"j \<le> USHORT_MAX" using a4 y1 by auto 
+  have y3:"j = len_ws_win - 1" using a3 ptr_offset_equality[OF y2 y1, where p="wsp +\<^sub>p int len_ws"] a4 by auto
+  have y4:" last win' = win' ! j" by (metis a2 a4 gr_implies_not0 last_conv_nth length_0_conv waypoints_window_aux_success_length y3)
+  have y5:"win = (butlast win') @ [nextwp_update (last win') (number_C (last win'))]" using a7 a2 waypoints_window_aux_to_waypoints_window_success_rel nextwp_update_def by auto
+  have y6:"win = (butlast win) @ [nextwp_update (win' ! j) (number_C (win' ! j))]" using y4 y5 by auto
+  have y7:"length win = len_ws_win"
+    by (metis (mono_tags, lifting) One_nat_def Suc_eq_plus1 Suc_pred' a2 a4 add.commute append_eq_append_conv dual_order.strict_trans1 eq_imp_le eq_refl gr_zeroI length_Cons length_append length_butlast length_neq list.size(3) not_less0 not_less_zero size_ne_size_imp_ne snoc_eq_iff_butlast waypoints_window_aux_success_length y3 y4 y4 y5 y6)
+  have y8:"win ! j = nextwp_update (win' ! j) (number_C (win' ! j))" using  y6 y7 y3 by (metis length_butlast nth_append_length)
+  thus ?thesis using y8 nextwp_update_def y3 a6 a4 by auto 
+qed
+      
+lemma GroomWindow_to_funspec_supp2:
+assumes a3:"Some win' = waypoints_window_aux (lift_waypoints s wsp len_ws) i len_ws_win"
+and a5:"Some win = waypoints_window ws i len_ws_win"
+and a8: "ws = lift_waypoints s wsp len_ws"
+and a10:"wsp +\<^sub>p int len_ws +\<^sub>p int j \<noteq> wsp +\<^sub>p int len_ws +\<^sub>p (int len_ws_win - 1)" 
+and a11:"j < len_ws_win"
+shows "win' ! j = win ! j"
+proof -
+  have y3:"j < len_ws_win - 1"  using a10 a11 nat_less_cases' by fastforce
+  thus ?thesis
+    by (metis (no_types, lifting) a11 a3 a5 a8 append_butlast_last_id length_butlast length_ineq_not_Nil(1) nth_append waypoints_window_aux_success_length waypoints_window_aux_to_waypoints_window_success_rel)
+qed
+      
+lemma GroomWindow_to_funspec:
+"(\<forall> (s::lifted_globals) v a. a < len_ws_win  \<longrightarrow> lift_waypoints (heap_Waypoint_struct_C_update (\<lambda>b c. if c =  wsp +\<^sub>p int len_ws +\<^sub>p int a then v b else b c) s) wsp len_ws = lift_waypoints s wsp len_ws)
+\<Longrightarrow> len_ws \<le> USHORT_MAX
+\<Longrightarrow> len_ws_win \<le> len_ws 
+\<Longrightarrow> 0<len_ws_win
+\<Longrightarrow> Some win' = waypoints_window_aux ws i len_ws_win \<Longrightarrow>
 \<lbrace>\<lambda> (s::lifted_globals).
-  are_valid_Waypoints s ws_winp len_ws_win
+  are_valid_Waypoints s (wsp +\<^sub>p len_ws) len_ws_win
   \<and> are_valid_Waypoints s wsp len_ws
   \<and> ws = lift_waypoints s wsp len_ws
- \<and> (\<forall> j. j <  len_ws_win \<longrightarrow> heap_Waypoint_struct_C s (ws_winp +\<^sub>p j) = win' ! j)
+ \<and> (\<forall> j. j <  len_ws_win \<longrightarrow> heap_Waypoint_struct_C s (wsp +\<^sub>p len_ws +\<^sub>p j) = win' ! j)
 \<rbrace>
-  LoadCode.MissionCommandUtils.GroomWindow' len_ws_win ws_winp
+  LoadCode.WaypointManagerUtils.GroomWindow' len_ws_win (wsp +\<^sub>p len_ws)
 \<lbrace> \<lambda> r s. 
-  are_valid_Waypoints s ws_winp len_ws_win
+  are_valid_Waypoints s (wsp +\<^sub>p len_ws) len_ws_win
   \<and> are_valid_Waypoints s wsp len_ws
   \<and> ws = lift_waypoints s wsp len_ws
   \<and> (\<exists> win. Some win = waypoints_window ws i len_ws_win
-    \<and> (\<forall> j. j <  len_ws_win \<longrightarrow> heap_Waypoint_struct_C s (ws_winp +\<^sub>p j) = win ! j)) \<rbrace>!"
-  sorry
+    \<and> (\<forall> j. j <  len_ws_win \<longrightarrow> heap_Waypoint_struct_C s (wsp +\<^sub>p len_ws +\<^sub>p j) = win ! j)) \<rbrace>!"
+  apply (subgoal_tac "len_ws_win - 1 < len_ws_win")
+  apply (subgoal_tac "\<exists> win. Some win = waypoints_window ws i len_ws_win")
+  apply (subgoal_tac "\<And> (s::lifted_globals) v.  lift_waypoints s wsp len_ws = lift_waypoints (heap_Waypoint_struct_C_update (\<lambda>b c. if c =  wsp +\<^sub>p int len_ws +\<^sub>p (int len_ws_win - 1) then v b else b c) s) wsp len_ws")
+  apply (unfold LoadCode.WaypointManagerUtils.GroomWindow'_def)
+  apply wp
+     apply (clarsimp | rule conjI impI)+
+      apply (rule exI[where x = "(butlast win' @ [nextwp_update (last win') (number_C (last win'))])"])
+     using lift_lift_waypoint_agnostic_prop[of "len_ws_win - 1"] apply (auto split: option.splits simp add: GroomWindow_to_funspec_supp1 GroomWindow_to_funspec_supp2)
+    by (metis (hide_lams) are_valid_Waypoints_def One_nat_def Suc_le_eq le_less neq0_conv of_nat_1 of_nat_diff zero_less_diff)+
 
 lemma FillAndGroomWaypoint_to_funspec:
 "len_ws \<le> USHORT_MAX
-\<Longrightarrow> ws_winp = wsp +\<^sub>p len_ws
 \<Longrightarrow> waypoints_wf ws
-\<Longrightarrow> Some win' = waypoints_window_aux ws i  len_ws_win
-\<Longrightarrow> len_ws_win < len_ws 
+\<Longrightarrow> Some win' = waypoints_window_aux ws i len_ws_win
+\<Longrightarrow> len_ws_win \<le> len_ws 
 \<Longrightarrow> 0<len_ws_win
-\<Longrightarrow> (\<forall> (s::lifted_globals) v a. a < len_ws_win  \<longrightarrow> lift_waypoints (heap_Waypoint_struct_C_update (\<lambda>b c. if c = ws_winp +\<^sub>p int a then v else b c) s) wsp len_ws = lift_waypoints s wsp len_ws)
+\<Longrightarrow> (\<forall> (s::lifted_globals) v a. a < len_ws_win  \<longrightarrow> lift_waypoints (heap_Waypoint_struct_C_update (\<lambda>b c. if c = wsp +\<^sub>p len_ws +\<^sub>p int a then v b else b c) s) wsp len_ws = lift_waypoints s wsp len_ws)
 \<Longrightarrow> \<lbrace>\<lambda> (s::lifted_globals).
-  are_valid_Waypoints s ws_winp len_ws_win
+  are_valid_Waypoints s (wsp +\<^sub>p len_ws) len_ws_win
   \<and> are_valid_Waypoints s wsp len_ws
   \<and> ws = lift_waypoints s wsp len_ws \<rbrace>
-  LoadCode.MissionCommandUtils.FillAndGroomWindow' wsp len_ws i len_ws_win ws_winp
+  LoadCode.WaypointManagerUtils.AutoPilotMissionCommandSegment' wsp len_ws i (wsp +\<^sub>p len_ws) len_ws_win 
 \<lbrace> \<lambda> r s. 
-  are_valid_Waypoints s ws_winp len_ws_win
+  are_valid_Waypoints s (wsp +\<^sub>p len_ws) len_ws_win
   \<and> are_valid_Waypoints s wsp len_ws
   \<and> ws = lift_waypoints s wsp len_ws
   \<and> (\<exists> win. Some win = waypoints_window ws i len_ws_win
-    \<and> (\<forall> j. j <  len_ws_win \<longrightarrow> heap_Waypoint_struct_C s (ws_winp +\<^sub>p j) = win ! j)) \<rbrace>!"
-  apply (unfold LoadCode.MissionCommandUtils.FillAndGroomWindow'_def)
+    \<and> (\<forall> j. j <  len_ws_win \<longrightarrow> heap_Waypoint_struct_C s (wsp +\<^sub>p len_ws +\<^sub>p j) = win ! j)) \<rbrace>!"
+  apply (unfold LoadCode.WaypointManagerUtils.AutoPilotMissionCommandSegment'_def)
   apply (rule validNF_nobind[where B="\<lambda> s. 
-  are_valid_Waypoints s ws_winp len_ws_win
+  are_valid_Waypoints s (wsp +\<^sub>p len_ws) len_ws_win
   \<and> are_valid_Waypoints s wsp len_ws
   \<and> ws = lift_waypoints s wsp len_ws
-  \<and> (\<forall> j. j <  len_ws_win \<longrightarrow> heap_Waypoint_struct_C s (ws_winp +\<^sub>p j) = win' ! j)"])
-   apply (rule foo)
-        apply (clarsimp | assumption )+ 
-   apply (rule FillWaypoint_to_funspec)
-       apply (clarsimp | assumption )+
-done
+  \<and> (\<forall> j. j <  len_ws_win \<longrightarrow> heap_Waypoint_struct_C s (wsp +\<^sub>p len_ws +\<^sub>p j) = win' ! j)"])
+  by (rule GroomWindow_to_funspec | clarsimp | assumption | rule FillWindow_to_funspec)+
     
 end
