sel4_artifacts/UxASSeL4/verification/LoadCode.thy
@@ -2,10 +2,26 @@ theory LoadCode imports
 "/home/dacosta/dev/rc/l4v/tools/autocorres/AutoCorres"
 begin
   
-install_C_file "../CMASI/MissionCommandUtils.c"
+install_C_file "./WaypointManagerUtils.c"
   
-autocorres[ts_rules = nondet, unsigned_word_abs = FillWindow FindWP GroomWindow FillAndGroomWindow ] "../CMASI/MissionCommandUtils.c"  
+autocorres[ts_rules = nondet, unsigned_word_abs = FillWindow FindWaypoint GroomWindow AutoPilotMissionCommandSegment ] "./WaypointManagerUtils.c"  
   
+
+(* IMPORTANT:
+ * The waypoint manager is going to at least store two array both with a maximum possible size of 
+ * 2^16-1. If the size of the waypoint data structure times 2*16-1 is not less than or equal to 
+ * the 2^32-1 Then we will no longer be able to gaurantee that a write to a mission command segment
+ * will not alter the original mission command.
+ * NB: I am assuming that maximum array size for LCMP messages is 2^16-1
+ *)
+lemma sanity_check_waypoint_size:"USHORT_MAX * size_of TYPE(Waypoint_struct_C) \<le> UINT_MAX"
+  apply(unfold USHORT_MAX_def UINT_MAX_def) by simp
+
+(* If the above lemma holds then this lemma will be true. Though I am not sure how to prove it. *)
+lemma ptr_offset_equality:"a \<le> USHORT_MAX \<Longrightarrow> b \<le> USHORT_MAX  \<Longrightarrow> (p::Waypoint_struct_C ptr) +\<^sub>p a = p +\<^sub>p b \<Longrightarrow> a = b"
+ apply(unfold ptr_add_def USHORT_MAX_def)
+ sorry
+
 
 (* A subset of what we expect a valid mission command to entail. I.E, the ptr to the front
  * of the waypoint pointer array is valid, all elements in that array are valid and all pointers
@@ -23,8 +39,8 @@ lemma valid_waypoints[simp]:
 \<Longrightarrow> is_valid_Waypoint_struct_C s (wsp +\<^sub>p j)"
   by (simp add: are_valid_Waypoints_def uint_nat word_less_nat_alt)
     
-(* Generally useful lemma." *)  
-lemma [simp]: "(a::32 word) < n \<Longrightarrow> unat (n - (a + 1)) < unat (n - a)"
+(* Generally useful lemma showing obvious things." *)  
+lemma loadcode1[simp]: "(a::32 word) < n \<Longrightarrow> unat (n - (a + 1)) < unat (n - a)"
 proof -
   assume "a < n"
   then have "0 \<noteq> n - a"
@@ -33,7 +49,7 @@ proof -
     by (simp add: add.commute diff_add_eq_diff_diff_swap measure_unat)
 qed
   
-lemma [simp]: "(a::16 word) < n \<Longrightarrow> unat (n - (a + 1)) < unat (n - a)"
+lemma loadcode2[simp]: "(a::16 word) < n \<Longrightarrow> unat (n - (a + 1)) < unat (n - a)"
 proof -
   assume "a < n"
   then have "0 \<noteq> n - a"
@@ -42,7 +58,7 @@ proof -
     by (simp add: add.commute diff_add_eq_diff_diff_swap measure_unat)
 qed
 
-lemma [simp]: "uint (a::16 word) < uint n \<Longrightarrow> unat (n - (a + 1)) < unat (n - a)"
+lemma loadcode3[simp]: "uint (a::16 word) < uint n \<Longrightarrow> unat (n - (a + 1)) < unat (n - a)"
 proof -
   assume "uint a < uint n"
   then have "0 \<noteq> n - a"
@@ -50,77 +66,88 @@ proof -
   then show ?thesis
     by (simp add: add.commute diff_add_eq_diff_diff_swap measure_unat)
 qed
-  
-lemma [simp]: "j < i \<Longrightarrow> int (unat j) = uint j" by (simp add: uint_nat)
-    
-lemma word16_leq_max_word16_as_int[simp]:"65535 \<le> x \<Longrightarrow> uint (a::16 word) \<le> x = True"
+lemma loadcode4[simp]:"65535 \<le> x \<Longrightarrow> uint (a::16 word) \<le> x = True"
   using word.uint[of a] by auto
     
-lemma [simp]:"i < 0 \<Longrightarrow> i < uint (j::16 word)"
+lemma loadcode5[simp]:"i < 0 \<Longrightarrow> i < uint (j::16 word)"
   by (metis less_trans neq_iff uint_lt_0)
     
-lemma [simp]:"INT_MIN < uint (len_ws_win::16 word)"
+lemma loadcode6[simp]:"INT_MIN < uint (len_ws_win::16 word)"
   using INT_MIN_def by fastforce
     
-lemma [simp]:"uint j < uint (x::16 word) - 1 \<Longrightarrow> j + 1 \<le> x"
+lemma loadcode7[simp]:"uint j < uint (x::16 word) - 1 \<Longrightarrow> j + 1 \<le> x"
   by (meson inc_le le_less word_less_def zle_diff1_eq)
-    
-
-lemma [simp]:"int USHORT_MAX \<le> 2147483646"
+ 
+lemma loadcode8[simp]:"int USHORT_MAX \<le> 2147483646"
 proof -
   have "int USHORT_MAX = 65535" using USHORT_MAX_def by auto
   thus ?thesis by auto
 qed    
 
-lemma [simp]:"uint (j::16 word) < uint (x::16 word) - 1 \<Longrightarrow> 0 < (j + 1)"
+lemma loadcode9[simp]:"uint (j::16 word) < uint (x::16 word) - 1 \<Longrightarrow> 0 < (j + 1)"
   by (metis (mono_tags, hide_lams) add.commute add_left_cancel le_less max_word_max not_less word_less_def word_neq_0_conv word_overflow zle_diff1_eq)
 
-lemma [simp]:"i \<le> 2147483645  \<Longrightarrow> int i < 2147483646"
+lemma loadcode10[simp]:"i \<le> 2147483645  \<Longrightarrow> int i < 2147483646"
   apply (induct i) by auto
-  
+
 lemma max_short_fix:"i \<le> USHORT_MAX \<Longrightarrow> int i < 2147483646"  
-sorry
-   
-lemma [simp]:"i \<le> USHORT_MAX \<Longrightarrow> uint ((of_nat i)::16 word) = int i"
-  sorry
+proof(induct i)
+  case 0
+  then show ?case by auto
+next
+  case (Suc i)
+  then have "i < 2147483646" by auto
+  then have "Suc i < 2147483646 \<or> Suc i = 2147483646" by auto
+  thus ?case
+  proof
+    assume "Suc i < 2147483646"
+    thus ?case by auto
+  next
+    assume "Suc i = 2147483646"
+    thus ?case using Suc by (simp add: USHORT_MAX_def)
+  qed
+qed
+    
+lemma loadcode11[simp]:"c \<le> USHORT_MAX \<Longrightarrow> b \<le> c \<Longrightarrow> a < b \<Longrightarrow> int a \<le> 2147483646"
+  by (meson le_less less_le_trans max_short_fix)
+
+lemma loadcode12[simp]:"(of_nat USHORT_MAX::16 word) = 65535"
+  apply (unfold of_nat_def USHORT_MAX_def)
+   by (metis of_nat_def of_nat_numeral)
+
+lemma loadcode13[simp]:"(65535::16 word) + 1 = 0"
+  by simp
+
+lemma loadcode14[simp]:"(i::16 word) + 1 = 0 \<Longrightarrow> i = 65535"
+  by (metis add.commute add_left_cancel loadcode13) 
+
+lemma loadcode15[simp]:"unat (0xffff::16 word) = USHORT_MAX"
+  apply (unfold of_nat_def USHORT_MAX_def) 
+  by simp
+    
+lemma loadcode16:"(i::16 word) + 1 = 0 \<Longrightarrow> unat i = USHORT_MAX"    
+  using loadcode14 loadcode15 by blast  
+    
+lemma loadcode17:"(i < ((of_nat USHORT_MAX)::16 word)) = (i < i + 1)"
+  apply auto
+  using less_is_non_zero_p1 word_overflow apply blast
+  by (metis le_less less_is_non_zero_p1 loadcode13 not_less)
+
+lemma loadcode18[simp]:"i \<le> USHORT_MAX \<Longrightarrow> unat (of_nat i::16 word) = i"
+  by (metis  le_unat_uoi loadcode15)
+
+lemma loadcode19[simp]:"i \<le> USHORT_MAX \<Longrightarrow> uint ((of_nat i)::16 word) = int i"
+  by (metis uint_nat loadcode18)
     
 lemma [simp]:"int len_ws_win \<le> 2147483648 \<Longrightarrow> 0 < len_ws_win \<Longrightarrow> int len_ws_win - 1 \<le> INT_MAX"
   sorry
 
-lemma rename1[simp]:"int len_ws_win \<le> 2147483648 \<Longrightarrow> 0 < len_ws_win \<Longrightarrow> uint (of_nat len_ws_win) - 1 \<le> INT_MAX"
+lemma rename2[simp]:"0 < a \<Longrightarrow> a \<le> INT_MAX \<Longrightarrow> uint (of_nat a) - 1 \<le> INT_MAX"
   sorry
-    
-lemma rename2[simp]:"0 < len_ws_win \<Longrightarrow> a \<le> USHORT_MAX \<Longrightarrow> uint (of_nat len_ws_win) - 1 \<le> INT_MAX"
-  sorry
-    
+
 lemma rename3[simp]:"len_ws \<le> USHORT_MAX \<Longrightarrow> len_ws_win \<le> len_ws \<Longrightarrow> int len_ws_win \<le> 2147483648"
    using max_short_fix by fastforce
-    
+   
 lemma [simp]:"0 < len_ws_win \<Longrightarrow> INT_MIN < int len_ws_win"
   sorry
-    
-lemma [simp]:"p +\<^sub>p int 0 = p"    
-  sorry
-
-lemma rename4[simp]:"(i::nat) < j \<Longrightarrow> \<not> int i < int j - 1 \<Longrightarrow> i = j - 1"
-  by linarith
-    
-lemma rename5[simp]:"a \<le> USHORT_MAX \<Longrightarrow> int a < 2147483648"
-  sorry
-
-lemma rename6[simp]:"a \<le> USHORT_MAX \<Longrightarrow> b \<le> a \<Longrightarrow> int b \<le> 2147483647"
-  sorry
-    
-lemma USHORT_MAX_LT_UINT_MAX[simp]:"x \<le> USHORT_MAX \<Longrightarrow> x \<le> UINT_MAX"
-  sorry
-    
-lemma noninter_pointer_add[simp]:"j \<le> USHORT_MAX \<Longrightarrow> 0 < j \<Longrightarrow> i < j \<Longrightarrow> ap +\<^sub>p i = ap +\<^sub>p j \<Longrightarrow> False"
-  sorry
-
-lemma rename7[simp,wp]:"a \<le> USHORT_MAX \<Longrightarrow> b < a  \<Longrightarrow> b \<le> 2147483648" 
-  sorry
-
-lemma rename8[simp,wp]:"a \<le> USHORT_MAX \<Longrightarrow> b < a - 1  \<Longrightarrow> int b \<le> 2147483646" 
-  sorry
-    
 end
